core/TofinoPipeline.v
@@ -1,0 +1,127 @@
+Require Import Poulet4.P4light.Syntax.P4defs.
+Require Import Poulet4.P4light.Semantics.Semantics.
+Require Import ProD3.core.Core.
+Require Import Poulet4.P4light.Architecture.Tofino.
+Require Import Poulet4.P4light.Architecture.Queue.
+Require Import Poulet4.P4light.Architecture.TrafficManager.
+Require Import Poulet4.P4light.Semantics.Typing.ValueTyping.
+Require Import ProD3.core.Tofino.
+
+Notation ident := string.
+Notation path := (list ident).
+Notation Val := (@ValueBase bool).
+Notation Sval := (@ValueBase (option bool)).
+Notation P4Type := (@P4Type Info).
+Notation packet := (list bool).
+Notation fundef := (@fundef Info).
+
+Section Pipeline.
+
+  Variable ge : (@genv _ target).
+
+  Inductive programmable_block :
+    path -> ident -> fundef -> Prop :=
+  | programmable_block_intro:
+    forall name fd pipe_class_name pipe_inst_path pipe_targs class_name inst_path targs,
+      PathMap.get ["main"; "pipe0"] (ge_inst ge) =
+        Some {|iclass:=pipe_class_name;
+               ipath:=pipe_inst_path; itargs:=pipe_targs|} ->
+      PathMap.get (pipe_inst_path ++ [name]) (ge_inst ge) =
+        Some {|iclass:=class_name; ipath:=inst_path; itargs:=targs|} ->
+      PathMap.get ([class_name; "apply"]) (ge_func ge) = Some fd ->
+      programmable_block inst_path name fd.
+
+  Definition programmable_block_sem :=
+    extern_state -> list Sval -> extern_state -> list Sval -> signal -> Prop.
+
+  (*
+  Inductive ingress_pipeline:
+    extern_state -> packet_in -> extern_state -> packet_out -> Sval -> Prop :=
+  | ingress_pipeline_intro:
+    forall inprsr_path inprsr ingress_path ingress indeprsr_path indeprsr pin pout
+      m1 m2 m3 m4 m5 m6 s0 s1 s2 s3 s4
+      hdr1 hdr2 hdr3 ig_md1 ig_md2
+      payload ig_intr_md ig_intr_md_from_prsr1 ig_intr_md_for_dprsr1
+      ig_intr_md_for_dprsr2 ig_intr_md_for_tm1 ig_intr_md_for_tm2,
+      PathMap.set ["packet_out"] (ObjPout [])
+        (PathMap.set ["packet_in"] (ObjPin pin) s0) = s1 ->
+      programmable_block inprsr_path "ingress_parser" inprsr ->
+      exec_func ge read_ndetbit inprsr_path (m1, s1) inprsr nil [] (m2, s2)
+        [hdr1; ig_md1; ig_intr_md; ig_intr_md_for_tm1; ig_intr_md_from_prsr1]
+        SReturnNull ->
+      PathMap.get ["packet_in"] s2 = Some (ObjPin payload) ->
+      programmable_block ingress_path "ingress" ingress ->
+      exec_func ge read_ndetbit ingress_path (m3, s2) ingress []
+        [hdr1; ig_md1; ig_intr_md; ig_intr_md_from_prsr1; ig_intr_md_for_dprsr1;
+         ig_intr_md_for_tm1] (m4, s3)
+        [hdr2; ig_md2; ig_intr_md_for_dprsr2; ig_intr_md_for_tm2] SReturnNull ->
+      programmable_block indeprsr_path "ingress_deparser" indeprsr ->
+      exec_func ge read_ndetbit indeprsr_path (m5, s3) indeprsr nil
+        [hdr2; ig_md2; ig_intr_md_for_dprsr2; ig_intr_md] (m6, s4) [hdr3]
+        SReturnNull ->
+      PathMap.get ["packet_out"] s4 = Some (ObjPout pout) ->
+      ingress_pipeline s0 pin s4 (pout ++ payload) ig_intr_md_for_tm2.
+
+  Inductive egress_pipeline:
+    extern_state -> packet_in -> extern_state -> packet_out -> Prop :=
+  | egress_pipeline_intro:
+    forall eprsr_path eprsr egress_path egress edeprsr_path edeprsr pin pout
+      m1 m2 m3 m4 m5 m6 s0 s1 s2 s3 s4 hdr1 hdr2 hdr3 hdr4 eg_md1 eg_md2 eg_intr_md
+      eg_intr_md_from_prsr payload eg_intr_md_for_dprsr1 eg_intr_md_for_dprsr2
+      eg_intr_md_for_oport1 eg_intr_md_for_oport2,
+      PathMap.set ["packet_out"] (ObjPout [])
+        (PathMap.set ["packet_in"] (ObjPin pin) s0) = s1 ->
+      programmable_block eprsr_path "ingress_parser" eprsr ->
+      exec_func ge read_ndetbit eprsr_path (m1, s1) eprsr nil [] (m2, s2)
+        [hdr1; eg_md1; eg_intr_md; eg_intr_md_from_prsr] SReturnNull ->
+      PathMap.get ["packet_in"] s2 = Some (ObjPin payload) ->
+      programmable_block egress_path "ingress" egress ->
+      exec_func ge read_ndetbit egress_path (m3, s2) egress nil
+        [hdr1; eg_md1; eg_intr_md; eg_intr_md_from_prsr; eg_intr_md_for_dprsr1;
+         eg_intr_md_for_oport1] (m4, s3)
+        [hdr2; eg_md2; eg_intr_md_for_dprsr2; eg_intr_md_for_oport2] SReturnNull ->
+      programmable_block edeprsr_path "ingress" edeprsr ->
+      exec_func ge read_ndetbit edeprsr_path (m5, s3) edeprsr nil
+        [hdr3; eg_md2; eg_intr_md_for_dprsr2; eg_intr_md; eg_intr_md_from_prsr]
+        (m6, s4) [hdr4] SReturnNull ->
+      PathMap.get ["packet_out"] s4 = Some (ObjPout pout) ->
+      egress_pipeline s0 pin s4 (pout ++ payload).
+*)
+
+End Pipeline.
+
+Inductive ingress_pipeline (inprsr ingress indeprsr: programmable_block_sem)
+  (parser_ingress_cond ingress_deprsr_cond: list Sval -> list Sval -> Prop) :
+  extern_state -> packet_in -> extern_state -> packet_out -> list Sval -> Prop :=
+| ingress_pipeline_intro:
+  forall pin pout s0 s1 s2 s3 s4 hdr1 hdr2 hdr3 ig_md1 ig_md2 payload
+    rest1 rest2 rest3 rest4 for_tm,
+    PathMap.set ["packet_out"] (ObjPout [])
+      (PathMap.set ["packet_in"] (ObjPin pin) s0) = s1 ->
+    inprsr s1 [] s2 (hdr1 :: ig_md1 :: rest1) SReturnNull ->
+    PathMap.get ["packet_in"] s2 = Some (ObjPin payload) ->
+    parser_ingress_cond rest1 rest2 ->
+    ingress s2 (hdr1 :: ig_md1 :: rest2) s3 (hdr2 :: ig_md2 :: rest3) SReturnNull ->
+    ingress_deprsr_cond rest3 rest4 ->
+    indeprsr s3 (hdr2 :: ig_md2 :: rest4) s4 [hdr3] SReturnNull ->
+    PathMap.get ["packet_out"] s4 = Some (ObjPout pout) ->
+    ingress_pipeline inprsr ingress indeprsr parser_ingress_cond
+      ingress_deprsr_cond s0 pin s4 (pout ++ payload) for_tm.
+
+Inductive egress_pipeline (eprsr egress edeprsr: programmable_block_sem)
+  (parser_egress_cond egress_deprsr_cond: list Sval -> list Sval -> Prop) :
+  extern_state -> packet_in -> extern_state -> packet_out -> Prop :=
+| egress_pipeline_intro:
+  forall pin pout s0 s1 s2 s3 s4 hdr1 hdr2 hdr3 hdr4 eg_md1 eg_md2 payload
+    rest1 rest2 rest3 rest4,
+    PathMap.set ["packet_out"] (ObjPout [])
+      (PathMap.set ["packet_in"] (ObjPin pin) s0) = s1 ->
+    eprsr s1 [] s2 (hdr1 :: eg_md1 :: rest1) SReturnNull ->
+    PathMap.get ["packet_in"] s2 = Some (ObjPin payload) ->
+    parser_egress_cond rest1 rest2 ->
+    egress s2 (hdr1 :: eg_md1 :: rest2) s3 (hdr2 :: eg_md2 :: rest3) SReturnNull ->
+    egress_deprsr_cond rest3 rest4 ->
+    edeprsr s3 (hdr3 :: eg_md2 :: rest4) s4 [hdr4] SReturnNull ->
+    PathMap.get ["packet_out"] s4 = Some (ObjPout pout) ->
+    egress_pipeline eprsr egress edeprsr parser_egress_cond egress_deprsr_cond
+      s0 pin s4 (pout ++ payload).
