examples/sampler/sampler_pipeline.v
@@ -1,0 +1,184 @@
+Require Import Poulet4.P4light.Syntax.P4defs.
+Require Import Poulet4.P4light.Semantics.Semantics.
+Require Import ProD3.core.Core.
+Require Import Poulet4.P4light.Architecture.Tofino.
+Require Import ProD3.core.Tofino.
+Require Import ProD3.core.TofinoPipeline.
+Require Import ProD3.examples.sampler.ModelRepr.
+Require Import ProD3.examples.sampler.common.
+Require Import ProD3.examples.sampler.verif_ingress_parser.
+Require Import ProD3.examples.sampler.verif_ingress.
+Require Import ProD3.examples.sampler.verif_ingress_deparser.
+Require Import ProD3.examples.sampler.verif_egress_parser.
+Require Import ProD3.examples.sampler.verif_egress.
+Require Import ProD3.examples.sampler.verif_egress_deparser.
+Require Import ProD3.core.ProgNotations.
+Require Import ProD3.core.PacketFormat.
+Require Import Poulet4.P4light.Syntax.P4Notations.
+Require Import Hammer.Plugin.Hammer.
+Require Export Coq.Program.Program.
+Import ListNotations.
+
+Definition extern_contains (es: extern_state) (p: path) (counter: Z) :=
+  PathMap.get (p ++ ["reg_count"]) es =
+      Some (ObjRegister [Z_to_val counter]) /\ 0 <= counter.
+
+Inductive inprsr_block: programmable_block_sem :=
+| parser_block_intro:
+  forall inst_path m m' es es' fd (pin pin': packet_in) ver port stamp ether ipv4 result
+    hdr ig_md ig_intr_md signal counter,
+    extern_contains es ["pipe"; "ingress"] counter ->
+    ⊫ᵥ iimt_repr_val 0 ver port stamp \: ingress_intrinsic_metadata_t ->
+    ⊫ᵥ ethernet_repr_val ether \: ethernet_h ->
+    ⊫ᵥ ipv4_repr_val ipv4 \: ipv4_h ->
+    (if is_tcp ipv4 then ⊫ᵥ result \: tcp_h else
+      (if is_udp ipv4 then ⊫ᵥ result \: udp_h else result = ValBaseNull)) ->
+      ethernet_ether_type ether = P4BitV 16 ETHERTYPE_IPV4 ->
+      pin ⫢ [⦑ encode (iimt_repr_val 0 ver port stamp) ⦒;
+             ⟨64⟩;
+             ⦑ encode (ethernet_repr_val ether) ⦒;
+             ⦑ encode (ipv4_repr_val ipv4) ⦒;
+             ⦃ is_tcp ipv4 ? ⦑ encode result ⦒ |
+               ⦃ is_udp ipv4 ? ⦑ encode result ⦒ | ε ⦄ ⦄; ⦑ pin' ⦒] ->
+      PathMap.get ["hdr"] m =
+        Some (common.hdr (sample_invalid_bridge hdr_init has_sample_init)) ->
+      PathMap.get ["packet_in"] es = Some (ObjPin pin) ->
+      programmable_block ge inst_path "ingress_parser" fd ->
+      extern_contains es' ["pipe"; "ingress"] counter ->
+      exec_func ge read_ndetbit inst_path (m, es) fd nil [] (m', es')
+        [hdr; ig_md; ig_intr_md] signal ->
+      inprsr_block es [] es' [hdr; ig_md; ig_intr_md] signal.
+
+Inductive ingress_block: programmable_block_sem :=
+| ingress_block_intro:
+  forall inst_path m m' es es' fd hdr1 hdr2 ig_md1 ig_md2 ig_intr_md
+    ig_intr_dprsr_md2 ig_intr_tm_md1 ig_intr_tm_md2 signal,
+    programmable_block ge inst_path "ingress" fd ->
+    let ig_intr_prsr_md :=
+      force ValBaseNull
+        (uninit_sval_of_typ None ingress_intrinsic_metadata_from_parser_t) in
+    let ig_intr_dprsr_md1 :=
+      force ValBaseNull
+        (uninit_sval_of_typ None ingress_intrinsic_metadata_for_deparser_t) in
+    exec_func ge read_ndetbit inst_path (m, es) fd nil
+      [hdr1; ig_md1; ig_intr_md; ig_intr_prsr_md;
+       ig_intr_dprsr_md1; ig_intr_tm_md1] (m', es')
+      [hdr2; ig_md2; ig_intr_dprsr_md2; ig_intr_tm_md2] signal ->
+    ingress_block es
+      [hdr1; ig_md1; ig_intr_md; ig_intr_prsr_md; ig_intr_dprsr_md1; ig_intr_tm_md1]
+      es' [hdr2; ig_md2; ig_intr_dprsr_md2; ig_intr_tm_md2] signal.
+
+Inductive indeprsr_block: programmable_block_sem :=
+| indeprsr_block_intro:
+  forall inst_path m m' es es' fd hdr1 hdr2 ig_md ig_intr_dprsr_md signal,
+    PathMap.get ["packet_out"] es = Some (ObjPout []) ->
+    programmable_block ge inst_path "ingress_deparser" fd ->
+    exec_func ge read_ndetbit inst_path (m, es) fd nil
+      [hdr1; ig_md; ig_intr_dprsr_md] (m', es') [hdr2] signal ->
+    indeprsr_block es [hdr1; ig_md; ig_intr_dprsr_md] es' [hdr2] signal.
+
+Inductive parser_ingress_cond: list Sval -> list Sval -> Prop :=
+| parser_ingress_cond_intro:
+  forall ig_intr_md ig_intr_prsr_md ig_intr_dprsr_md ig_intr_tm_md,
+    parser_ingress_cond [ig_intr_md]
+      [ig_intr_md; ig_intr_prsr_md; ig_intr_dprsr_md; ig_intr_tm_md].
+
+Inductive ingress_deprsr_cond: list Sval -> list Sval -> Prop :=
+| ingress_deprsr_cond_intro:
+  forall ig_intr_dprsr_md ig_intr_tm_md,
+    ingress_deprsr_cond [ig_intr_dprsr_md; ig_intr_tm_md] [ig_intr_dprsr_md].
+
+Lemma get_packet: forall v1 v2 (es: extern_state),
+    PathMap.get ["packet_in"]
+      (PathMap.set ["packet_out"] v1 (PathMap.set ["packet_in"] v2 es)) = Some v2.
+Proof.
+  intros. rewrite PathMap.get_set_diff; [|intro HS; inversion HS].
+  rewrite PathMap.get_set_same. reflexivity.
+Qed.
+
+Lemma ethernet_extract_result_hdr:
+  forall (ether : ethernet_rec) (ipv4 : ipv4_rec) (result : Val),
+  exists (ethernet tcp udp : Sval) (ip4 : ipv4_rec),
+    ethernet_extract_result
+      (common.hdr (sample_valid_bridge hdr_init has_sample_init)) ether ipv4
+      result = hdr ethernet tcp udp ip4.
+Proof.
+  intros ether ipv4 result.
+  unfold ethernet_extract_result. unfold protocol_extract_result.
+  unfold sample_valid_bridge, hdr_init, has_sample_init. simpl. unfold hdr.
+  destruct (is_tcp ipv4); [do 4 eexists; reflexivity |].
+  destruct (is_udp ipv4); [do 4 eexists; reflexivity |].
+  do 4 eexists; reflexivity.
+Qed.
+
+Lemma sval_refine_iimt_repr_sval: forall ver port stamp,
+  sval_refine
+    (force ValBaseNull (uninit_sval_of_typ None ingress_intrinsic_metadata_t))
+    (iimt_repr_sval 0 ver port stamp).
+Proof.
+  intros. unfold iimt_repr_sval. simpl. constructor. constructor.
+  do 6 (constructor; [simpl; split; [reflexivity | repeat constructor]|]).
+  constructor.
+Qed.
+
+Lemma counter_iff:
+  forall (s : extern_state) (counter : Z) pa,
+    extern_contains s pa counter <-> counter_repr pa counter s.
+Proof.
+  intros. unfold counter_repr. split; intros.
+  - hnf. split; [|simpl; auto]. destruct H. hnf. split; simpl; assumption.
+  - hnf in H. destruct H as [H _]. hnf in H. simpl in H.
+    destruct H. split; assumption.
+Qed.
+
+Lemma hdr_exists: forall ethernet tcp udp ip4,
+  exists h, hdr ethernet tcp udp ip4 = eval_val_to_sval h /\
+         ⊢ᵥ h \: header_sample_t.
+Proof.
+  intros. eexists. split.
+  - unfold hdr.
+Abort.
+
+Lemma process_packet_ingress:
+  forall es es' pin pout for_tm,
+    ingress_pipeline
+      inprsr_block ingress_block indeprsr_block parser_ingress_cond
+      ingress_deprsr_cond es pin es' pout for_tm -> False.
+Proof.
+  intros. inversion H. subst. inv H1. rewrite get_packet in H18.
+  inversion H18. subst pin0; clear H18. inv H20. inv H0. inv H1. inv H8.
+  eapply (proj1 ingress_parser_body) in H24; eauto.
+  2: { hnf. split. 1: constructor. hnf. split.
+       - hnf. simpl. rewrite H17. split; auto. apply sval_refine_refl.
+       - hnf. simpl. rewrite get_packet. intuition. }
+  destruct H24. hnf in H0. inv H0. inv H21. inv H23. clear H24.
+  destruct H1 as [_ [_ [H1 _]]]. hnf in H1. rewrite H1 in H2.
+  inv H2. inv H4. inv H3. inv H27. inv H0. inv H2. inv H3.
+  destruct (ethernet_extract_result_hdr ether ipv4 result) as
+    [ethernet [tcp [udp [ip4 ?H]]]]. rewrite H0 in H19.
+  eapply (proj1 ingress_body counter ethernet
+            tcp udp ip4 ig_intr_tm_md1) in H28; eauto.
+  2: { split.
+       - hnf. do 2 (constructor; [assumption |]).
+         constructor.
+         1: { apply sval_refine_trans with (iimt_repr_sval 0 ver port stamp).
+              2: assumption. apply sval_refine_iimt_repr_sval. }
+         subst ig_intr_prsr_md. constructor; [apply sval_refine_refl|].
+         subst ig_intr_dprsr_md1. constructor; [apply sval_refine_refl|].
+         constructor; [apply sval_refine_refl | constructor].
+       - split. hnf. auto. hnf. split. 2: simpl; auto.
+         rewrite <- counter_iff. assumption. }
+  destruct H28. hnf in H2. inv H2. inv H24. inv H25. inv H26. clear H27.
+  destruct H3 as [_ [_ [H3 _]]]. rewrite <- counter_iff in H3.
+  inv H6. inv H5. inv H30. inv H2. inv H4. inv H5.
+  eapply (proj1 ingress_deparser_body []) in H31; eauto.
+  3: { split.
+       - hnf. constructor.
+         apply sval_refine_trans with
+           (if counter mod 1024 =? 0
+           then update_hdr ethernet tcp udp ip4 (counter + 1)
+           else hdr ethernet tcp udp ip4). 2: assumption.
+         admit. constructor. apply H9.
+         constructor. apply H23. constructor.
+       - split. 1: hnf; auto. hnf. split. 2: simpl; auto. simpl. assumption. }
+Abort.
